removed Cell from Map_Get and Map_Put

Source/Concurrency/LinearRewriter.cs
@@ -451,7 +451,8 @@ public class LinearRewriter
     var cmdSeq = new List<Cmd>();
     var path = callCmd.Ins[0];
     var k = callCmd.Ins[1];
-    var c = callCmd.Outs[0];
+    var l = callCmd.Outs[0];
+    var v = callCmd.Outs[1];
 
     var instantiation = monomorphizer.GetTypeInstantiation(callCmd.Proc);
     var domain = instantiation["K"];
@@ -460,9 +461,9 @@ public class LinearRewriter
     var mapRemoveFunc = MapRemove(domain, range);
     var mapAtFunc = MapAt(domain, range);
     cmdSeq.Add(AssertCmd(callCmd.tok, ExprHelper.FunctionCall(mapContainsFunc, path, k), "Map_Get failed"));
-    var cellConstructor = CellConstructor(domain, range);
-    cmdSeq.Add(
-      CmdHelper.AssignCmd(c.Decl, ExprHelper.FunctionCall(cellConstructor, k, ExprHelper.FunctionCall(mapAtFunc, path, k))));
+    var oneConstructor = OneConstructor(domain);
+    cmdSeq.Add(CmdHelper.AssignCmd(l.Decl, ExprHelper.FunctionCall(oneConstructor, k)));
+    cmdSeq.Add(CmdHelper.AssignCmd(v.Decl, ExprHelper.FunctionCall(mapAtFunc, path, k)));
     cmdSeq.Add(
       CmdHelper.AssignCmd(CmdHelper.ExprToAssignLhs(path), ExprHelper.FunctionCall(mapRemoveFunc, path, k)));
 
@@ -474,7 +475,8 @@ public class LinearRewriter
   {
     var cmdSeq = new List<Cmd>();
     var path = callCmd.Ins[0];
-    var c = callCmd.Ins[1];
+    var l = callCmd.Ins[1];
+    var v = callCmd.Ins[2];
 
     var instantiation = monomorphizer.GetTypeInstantiation(callCmd.Proc);
     var domain = instantiation["K"];
@@ -482,9 +484,9 @@ public class LinearRewriter
     var mapContainsFunc = MapContains(domain, range);
     var mapUpdateFunc = MapUpdate(domain, range);
     var attribute = new QKeyValue(Token.NoToken, "linear", new List<object>(), null);
-    cmdSeq.Add(new AssumeCmd(Token.NoToken, Expr.Not(ExprHelper.FunctionCall(mapContainsFunc, path, Key(c))), attribute));
+    cmdSeq.Add(new AssumeCmd(Token.NoToken, Expr.Not(ExprHelper.FunctionCall(mapContainsFunc, path, Val(l))), attribute));
     cmdSeq.Add(
-      CmdHelper.AssignCmd(CmdHelper.ExprToAssignLhs(path), ExprHelper.FunctionCall(mapUpdateFunc, path, Key(c), Val(c))));
+      CmdHelper.AssignCmd(CmdHelper.ExprToAssignLhs(path), ExprHelper.FunctionCall(mapUpdateFunc, path, Val(l), v)));
 
     ResolveAndTypecheck(options, cmdSeq);
     return cmdSeq;
