Test/civl/samples/treiber-stack.bpl
@@ -6,11 +6,10 @@ function {:inline} AllLocPieces(): Set LocPiece {
   Set_Add(Set_Add(Set_Empty(), Left()), Right())
 }
 
-type TreiberNode _;
-type LocTreiberNode T = Fraction Loc LocPiece;
-type StackElem T = Node (LocTreiberNode T) T;
-type StackMap T = Map (LocTreiberNode T) (StackElem T);
-datatype Treiber<T> { Treiber(top: Option (LocTreiberNode T), {:linear} stack: StackMap T) }
+type LocTreiberNode = Fraction Loc LocPiece;
+type StackElem T = Node LocTreiberNode T;
+type StackMap T = Map LocTreiberNode (StackElem T);
+datatype Treiber<T> { Treiber(top: Option LocTreiberNode, {:linear} stack: StackMap T) }
 
 type X; // module type parameter
 
@@ -19,7 +18,7 @@ var {:layer 0, 4} {:linear} ts: Map Loc (Treiber X);
 
 /// Yield invariants
 
-function {:inline} Domain(ts: Map Loc (Treiber X), loc_t: Loc): Set (LocTreiberNode X) {
+function {:inline} Domain(ts: Map Loc (Treiber X), loc_t: Loc): Set LocTreiberNode {
   ts->val[loc_t]->stack->dom
 }
 
@@ -28,14 +27,14 @@ yield invariant {:layer 1} Yield();
 yield invariant {:layer 2} TopInStack(loc_t: Loc);
 invariant Map_Contains(ts, loc_t);
 invariant (var loc_n := Map_At(ts, loc_t)->top; loc_n is None || Set_Contains(Domain(ts, loc_t), loc_n->t));
-invariant (forall loc_n: LocTreiberNode X :: Set_Contains(Domain(ts, loc_t), loc_n) ==> 
+invariant (forall loc_n: LocTreiberNode :: Set_Contains(Domain(ts, loc_t), loc_n) ==>
               (var loc_n' := Map_At(Map_At(ts, loc_t)->stack, loc_n)->next; loc_n' is None || Set_Contains(Domain(ts, loc_t), loc_n'->t)));
 
-yield invariant {:layer 2} LocInStackOrNone(loc_t: Loc, loc_n: Option (LocTreiberNode X));
+yield invariant {:layer 2} LocInStackOrNone(loc_t: Loc, loc_n: Option LocTreiberNode);
 invariant Map_Contains(ts, loc_t);
 invariant loc_n is None || Set_Contains(Domain(ts, loc_t), loc_n->t);
 
-yield invariant {:layer 3} LocInStack(loc_t: Loc, loc_n: LocTreiberNode X);
+yield invariant {:layer 3} LocInStack(loc_t: Loc, loc_n: LocTreiberNode);
 invariant Map_Contains(ts, loc_t);
 invariant Set_Contains(Domain(ts, loc_t), loc_n);
 
@@ -44,7 +43,7 @@ invariant Map_Contains(ts, loc_t);
 invariant (var t := ts->val[loc_t]; Between(t->stack->val, t->top, t->top, None()));
 invariant (var t := ts->val[loc_t]; IsSubset(BetweenSet(t->stack->val, t->top, None()), Domain(ts, loc_t)->val));
 invariant (var loc_n := Map_At(ts, loc_t)->top; loc_n is None || Set_Contains(Domain(ts, loc_t), loc_n->t));
-invariant (forall {:pool "A"} loc_n: LocTreiberNode X :: {:add_to_pool "A", loc_n} Set_Contains(Domain(ts, loc_t), loc_n) ==>
+invariant (forall {:pool "A"} loc_n: LocTreiberNode :: {:add_to_pool "A", loc_n} Set_Contains(Domain(ts, loc_t), loc_n) ==>
               loc_n == Fraction(loc_n->val, Left(), AllLocPieces()) &&
               (var loc_n' := Map_At(Map_At(ts, loc_t)->stack, loc_n)->next; loc_n' is None || Set_Contains(Domain(ts, loc_t), loc_n'->t)));
 invariant Map_At(Stack, loc_t) == Abs(Map_At(ts, loc_t));
@@ -53,7 +52,7 @@ yield invariant {:layer 4} StackDom();
 invariant Stack->dom == ts->dom;
 
 yield invariant {:layer 4} PushLocInStack(
-  loc_t: Loc, node: StackElem X, new_loc_n: LocTreiberNode X, {:linear} right_loc_piece: One (LocTreiberNode X));
+  loc_t: Loc, node: StackElem X, new_loc_n: LocTreiberNode, {:linear} right_loc_piece: One LocTreiberNode);
 invariant Map_Contains(ts, loc_t);
 invariant Set_Contains(Domain(ts, loc_t), new_loc_n);
 invariant right_loc_piece->val == Fraction(new_loc_n->val, Right(), AllLocPieces());
@@ -76,19 +75,17 @@ yield procedure {:layer 4} Alloc() returns (loc_t: Loc)
 refines AtomicAlloc;
 preserves call StackDom();
 {
-  var top: Option (LocTreiberNode X);
+  var top: Option LocTreiberNode;
   var {:linear} stack: StackMap X;
   var {:linear} treiber: Treiber X;
   var {:linear} one_loc_t: One Loc;
-  var {:linear} cell_t: Cell Loc (Treiber X);
 
   top := None();
   call stack := Map_MakeEmpty();
   treiber := Treiber(top, stack);
   call one_loc_t := Loc_New();
-  call cell_t := Cell_Pack(one_loc_t, treiber);
   loc_t := one_loc_t->val;
-  call AllocTreiber#0(cell_t);
+  call AllocTreiber#0(one_loc_t, treiber);
   call {:layer 4} Stack := Copy(Map_Update(Stack, loc_t, Vec_Empty()));
   call {:layer 4} AbsLemma(treiber);
 }
@@ -109,9 +106,9 @@ preserves call TopInStack(loc_t);
 preserves call ReachInStack(loc_t);
 preserves call StackDom();
 {
-  var loc_n: Option (LocTreiberNode X);
-  var new_loc_n: LocTreiberNode X;
-  var {:linear} right_loc_piece: One (LocTreiberNode X);
+  var loc_n: Option LocTreiberNode;
+  var new_loc_n: LocTreiberNode;
+  var {:linear} right_loc_piece: One LocTreiberNode;
   var {:layer 4} old_treiber: Treiber X;
 
   call {:layer 4} old_treiber := Copy(ts->val[loc_t]);
@@ -160,22 +157,19 @@ preserves call StackDom();
 }
 
 atomic action {:layer 4} AtomicAllocNode#3(loc_t: Loc, x: X)
-  returns (loc_n: Option (LocTreiberNode X), new_loc_n: LocTreiberNode X, {:linear} right_loc_piece: One (LocTreiberNode X))
+  returns (loc_n: Option LocTreiberNode, new_loc_n: LocTreiberNode, {:linear} right_loc_piece: One LocTreiberNode)
 modifies ts;
 asserts Map_Contains(ts, loc_t);
 {
   var {:linear} one_loc_t: One Loc;
   var {:linear} treiber: Treiber X;
-  var top: Option (LocTreiberNode X);
+  var top: Option LocTreiberNode;
   var {:linear} stack: StackMap X;
   var {:linear} one_loc_n: One Loc;
-  var {:linear} cell_n: Cell (LocTreiberNode X) (StackElem X);
-  var {:linear} cell_t: Cell Loc (Treiber X);
-  var {:linear} loc_pieces: Set (Fraction Loc LocPiece);
-  var {:linear} left_loc_piece: One (Fraction Loc LocPiece);
+  var {:linear} loc_pieces: Set LocTreiberNode;
+  var {:linear} left_loc_piece: One LocTreiberNode;
   
-  call cell_t := Map_Get(ts, loc_t);
-  call one_loc_t, treiber := Cell_Unpack(cell_t);
+  call one_loc_t, treiber := Map_Get(ts, loc_t);
   Treiber(top, stack) := treiber;
   assume loc_n is None || Map_Contains(stack, loc_n->t);
   call one_loc_n := Loc_New();
@@ -183,22 +177,19 @@ asserts Map_Contains(ts, loc_t);
   call left_loc_piece := One_Get(loc_pieces, Fraction(one_loc_n->val, Left(), AllLocPieces()));
   new_loc_n := left_loc_piece->val;
   call right_loc_piece := One_Get(loc_pieces, Fraction(one_loc_n->val, Right(), AllLocPieces()));
-  call cell_n := Cell_Pack(left_loc_piece, Node(loc_n, x));
-  call Map_Put(stack, cell_n);
+  call Map_Put(stack, left_loc_piece, Node(loc_n, x));
   treiber := Treiber(top, stack);
-  call cell_t := Cell_Pack(one_loc_t, treiber);
-  call Map_Put(ts, cell_t);
+  call Map_Put(ts, one_loc_t, treiber);
 }
 yield procedure {:layer 3} AllocNode#3(loc_t: Loc, x: X)
-  returns (loc_n: Option (LocTreiberNode X), new_loc_n: LocTreiberNode X, {:linear} right_loc_piece: One (LocTreiberNode X))
+  returns (loc_n: Option LocTreiberNode, new_loc_n: LocTreiberNode, {:linear} right_loc_piece: One LocTreiberNode)
 preserves call TopInStack(loc_t);
 ensures call LocInStackOrNone(loc_t, Some(new_loc_n));
 refines AtomicAllocNode#3;
 {
   var {:linear} one_loc_n: One Loc;
-  var {:linear} cell_n: Cell (LocTreiberNode X) (StackElem X);
-  var {:linear} loc_pieces: Set (Fraction Loc LocPiece);
-  var {:linear} left_loc_piece: One (Fraction Loc LocPiece);
+  var {:linear} loc_pieces: Set LocTreiberNode;
+  var {:linear} left_loc_piece: One LocTreiberNode;
 
   call loc_n := ReadTopOfStack#Push(loc_t);
   call one_loc_n := Loc_New();
@@ -206,31 +197,27 @@ refines AtomicAllocNode#3;
   call left_loc_piece := One_Get(loc_pieces, Fraction(one_loc_n->val, Left(), AllLocPieces()));
   new_loc_n := left_loc_piece->val;
   call right_loc_piece := One_Get(loc_pieces, Fraction(one_loc_n->val, Right(), AllLocPieces()));
-  call cell_n := Cell_Pack(left_loc_piece, Node(loc_n, x));
-  call AllocNode#0(loc_t, cell_n);
+  call AllocNode#0(loc_t, left_loc_piece, Node(loc_n, x));
 }
 
 atomic action {:layer 4} AtomicPopIntermediate(loc_t: Loc) returns (success: bool, x_opt: Option X)
 modifies ts;
 {
   var {:linear} one_loc_t: One Loc;
-  var loc_n: Option (LocTreiberNode X);
+  var loc_n: Option LocTreiberNode;
   var {:linear} treiber: Treiber X;
-  var top: Option (LocTreiberNode X);
+  var top: Option LocTreiberNode;
   var {:linear} stack: StackMap X;
-  var {:linear} cell_t: Cell Loc (Treiber X);
   var x: X;
 
   assert Map_Contains(ts, loc_t);
   if (*) {
-    call cell_t := Map_Get(ts, loc_t);
-    call one_loc_t, treiber := Cell_Unpack(cell_t);
+    call one_loc_t, treiber := Map_Get(ts, loc_t);
     Treiber(top, stack) := treiber;
     assume top is Some && Map_Contains(stack, top->t);
     Node(loc_n, x) := Map_At(stack, top->t);
     treiber := Treiber(loc_n, stack);
-    call cell_t := Cell_Pack(one_loc_t, treiber);
-    call Map_Put(ts, cell_t);
+    call Map_Put(ts, one_loc_t, treiber);
     x_opt := Some(x);
     success := true;
   }
@@ -247,7 +234,7 @@ yield procedure {:layer 3} PopIntermediate(loc_t: Loc) returns (success: bool, x
 refines AtomicPopIntermediate;
 preserves call TopInStack(loc_t);
 {
-  var loc_n, new_loc_n: Option (LocTreiberNode X);
+  var loc_n, new_loc_n: Option LocTreiberNode;
   var node: StackElem X;
   var x: X;
 
@@ -269,12 +256,12 @@ preserves call TopInStack(loc_t);
   }
 }
 
-right action {:layer 3} AtomicReadTopOfStack#Push(loc_t: Loc) returns (loc_n: Option (LocTreiberNode X))
+right action {:layer 3} AtomicReadTopOfStack#Push(loc_t: Loc) returns (loc_n: Option LocTreiberNode)
 {
   assert Map_Contains(ts, loc_t);
   assume loc_n is None || Set_Contains(Domain(ts, loc_t), loc_n->t);
 }
-yield procedure {:layer 2} ReadTopOfStack#Push(loc_t: Loc) returns (loc_n: Option (LocTreiberNode X))
+yield procedure {:layer 2} ReadTopOfStack#Push(loc_t: Loc) returns (loc_n: Option LocTreiberNode)
 preserves call TopInStack(loc_t);
 ensures call LocInStackOrNone(loc_t, loc_n);
 refines AtomicReadTopOfStack#Push;
@@ -282,12 +269,12 @@ refines AtomicReadTopOfStack#Push;
   call loc_n := ReadTopOfStack#0(loc_t);
 }
 
-atomic action {:layer 3} AtomicReadTopOfStack#Pop(loc_t: Loc) returns (loc_n: Option (LocTreiberNode X))
+atomic action {:layer 3} AtomicReadTopOfStack#Pop(loc_t: Loc) returns (loc_n: Option LocTreiberNode)
 {
   assert Map_Contains(ts, loc_t);
   assume if loc_n is None then Map_At(ts, loc_t)->top is None else Set_Contains(Domain(ts, loc_t), loc_n->t);
 }
-yield procedure {:layer 2} ReadTopOfStack#Pop(loc_t: Loc) returns (loc_n: Option (LocTreiberNode X))
+yield procedure {:layer 2} ReadTopOfStack#Pop(loc_t: Loc) returns (loc_n: Option LocTreiberNode)
 preserves call TopInStack(loc_t);
 ensures call LocInStackOrNone(loc_t, loc_n);
 refines AtomicReadTopOfStack#Pop;
@@ -295,7 +282,7 @@ refines AtomicReadTopOfStack#Pop;
   call loc_n := ReadTopOfStack#0(loc_t);
 }
 
-right action {:layer 2,3} AtomicLoadNode#1(loc_t: Loc, loc_n: LocTreiberNode X) returns (node: StackElem X)
+right action {:layer 2,3} AtomicLoadNode#1(loc_t: Loc, loc_n: LocTreiberNode) returns (node: StackElem X)
 {
   assert Map_Contains(ts, loc_t);
   assert Map_Contains(Map_At(ts, loc_t)->stack, loc_n);
@@ -304,93 +291,78 @@ right action {:layer 2,3} AtomicLoadNode#1(loc_t: Loc, loc_n: LocTreiberNode X) 
 
 /// Primitives
 
-atomic action {:layer 1} AtomicLoadNode#0(loc_t: Loc, loc_n: LocTreiberNode X) returns (node: StackElem X)
+atomic action {:layer 1} AtomicLoadNode#0(loc_t: Loc, loc_n: LocTreiberNode) returns (node: StackElem X)
 modifies ts;
 refines AtomicLoadNode#1;
 {
   var {:linear} one_loc_t: One Loc;
   var {:linear} treiber: Treiber X;
-  var {:linear} cell_t: Cell Loc (Treiber X);
-  var top: Option (LocTreiberNode X);
+  var top: Option LocTreiberNode;
   var {:linear} stack: StackMap X;
-  var {:linear} one_loc_n: One (LocTreiberNode X);
-  var {:linear} cell_n: Cell (LocTreiberNode X) (StackElem X);
+  var {:linear} one_loc_n: One LocTreiberNode;
 
-  call cell_t := Map_Get(ts, loc_t);
-  call one_loc_t, treiber := Cell_Unpack(cell_t);
+  call one_loc_t, treiber := Map_Get(ts, loc_t);
   Treiber(top, stack) := treiber;
-  call cell_n := Map_Get(stack, loc_n);
-  call one_loc_n, node := Cell_Unpack(cell_n);
-  call cell_n := Cell_Pack(one_loc_n, node);
-  call Map_Put(stack, cell_n);
+  call one_loc_n, node := Map_Get(stack, loc_n);
+  call Map_Put(stack, one_loc_n, node);
   treiber := Treiber(top, stack);
-  call cell_t := Cell_Pack(one_loc_t, treiber);
-  call Map_Put(ts, cell_t);
+  call Map_Put(ts, one_loc_t, treiber);
 }
-yield procedure {:layer 0} LoadNode#0(loc_t: Loc, loc_n: LocTreiberNode X) returns (node: StackElem X);
+yield procedure {:layer 0} LoadNode#0(loc_t: Loc, loc_n: LocTreiberNode) returns (node: StackElem X);
 refines AtomicLoadNode#0;
 
-atomic action {:layer 1,2} AtomicReadTopOfStack#0(loc_t: Loc) returns (loc_n: Option (LocTreiberNode X))
+atomic action {:layer 1,2} AtomicReadTopOfStack#0(loc_t: Loc) returns (loc_n: Option LocTreiberNode)
 modifies ts;
 {
   var {:linear} one_loc_t: One Loc;
   var {:linear} treiber: Treiber X;
-  var {:linear} cell_t: Cell Loc (Treiber X);
 
-  call cell_t := Map_Get(ts, loc_t);
-  call one_loc_t, treiber := Cell_Unpack(cell_t);
+  call one_loc_t, treiber := Map_Get(ts, loc_t);
   loc_n := treiber->top;
-  call cell_t := Cell_Pack(one_loc_t, treiber);
-  call Map_Put(ts, cell_t);
+  call Map_Put(ts, one_loc_t, treiber);
 }
-yield procedure {:layer 0} ReadTopOfStack#0(loc_t: Loc) returns (loc_n: Option (LocTreiberNode X));
+yield procedure {:layer 0} ReadTopOfStack#0(loc_t: Loc) returns (loc_n: Option LocTreiberNode);
 refines AtomicReadTopOfStack#0;
 
 atomic action {:layer 1,4} AtomicWriteTopOfStack#0(
-  loc_t: Loc, old_loc_n: Option (LocTreiberNode X), new_loc_n: Option (LocTreiberNode X)) returns (success: bool)
+  loc_t: Loc, old_loc_n: Option LocTreiberNode, new_loc_n: Option LocTreiberNode) returns (success: bool)
 modifies ts;
 {
   var {:linear} treiber: Treiber X;
-  var {:linear} cell_t: Cell Loc (Treiber X);
   var {:linear} one_loc_t: One Loc;
 
-  call cell_t := Map_Get(ts, loc_t);
-  call one_loc_t, treiber := Cell_Unpack(cell_t);
+  call one_loc_t, treiber := Map_Get(ts, loc_t);
   if (old_loc_n == treiber->top) {
     treiber->top := new_loc_n;
     success := true;
   } else {
     success := false;
   }
-  call cell_t := Cell_Pack(one_loc_t, treiber);
-  call Map_Put(ts, cell_t);
+  call Map_Put(ts, one_loc_t, treiber);
 }
 yield procedure {:layer 0} WriteTopOfStack#0(
-  loc_t: Loc, old_loc_n: Option (LocTreiberNode X), new_loc_n: Option (LocTreiberNode X)) returns (success: bool);
+  loc_t: Loc, old_loc_n: Option LocTreiberNode, new_loc_n: Option LocTreiberNode) returns (success: bool);
 refines AtomicWriteTopOfStack#0;
 
-atomic action {:layer 1,3} AtomicAllocNode#0(loc_t: Loc, {:linear_in} cell_n: Cell (LocTreiberNode X) (StackElem X))
+atomic action {:layer 1,3} AtomicAllocNode#0(loc_t: Loc, {:linear_in} loc_piece: One LocTreiberNode, node: StackElem X)
 modifies ts;
 {
   var {:linear} one_loc_t: One Loc;
   var {:linear} treiber: Treiber X;
-  var {:linear} cell_t: Cell Loc (Treiber X);
 
-  call cell_t := Map_Get(ts, loc_t);
-  call one_loc_t, treiber := Cell_Unpack(cell_t);
-  call Map_Put(treiber->stack, cell_n);
-  call cell_t := Cell_Pack(one_loc_t, treiber);
-  call Map_Put(ts, cell_t);
+  call one_loc_t, treiber := Map_Get(ts, loc_t);
+  call Map_Put(treiber->stack, loc_piece, node);
+  call Map_Put(ts, one_loc_t, treiber);
 }
-yield procedure {:layer 0} AllocNode#0(loc_t: Loc, {:linear_in} cell_n: Cell (LocTreiberNode X) (StackElem X));
+yield procedure {:layer 0} AllocNode#0(loc_t: Loc, {:linear_in} loc_piece: One LocTreiberNode, node: StackElem X);
 refines AtomicAllocNode#0;
 
-atomic action {:layer 1,4} AtomicAllocTreiber#0({:linear_in} cell_t: Cell Loc (Treiber X))
+atomic action {:layer 1,4} AtomicAllocTreiber#0({:linear_in} one_loc_t: One Loc, {:linear_in} treiber: Treiber X)
 modifies ts;
 {
-  call Map_Put(ts, cell_t);
+  call Map_Put(ts, one_loc_t, treiber);
 }
-yield procedure {:layer 0} AllocTreiber#0({:linear_in} cell_t: Cell Loc (Treiber X));
+yield procedure {:layer 0} AllocTreiber#0({:linear_in} one_loc_t: One Loc, {:linear_in} treiber: Treiber X);
 refines AtomicAllocTreiber#0;
 
 /// Proof of abstraction with a manual encoding of termination
@@ -417,7 +389,7 @@ ensures absStack == AbsDefinition(treiber');
 free ensures absStack == Abs(treiber);
 free ensures absStack == Abs(treiber');
 {
-  var loc_n: Option (LocTreiberNode X);
+  var loc_n: Option LocTreiberNode;
   var n: StackElem X;
 
   if (treiber->top == None()) {
